bedrock2/src/bedrock2Examples/swap.v
@@ -19,34 +19,37 @@ Definition swap_swap := func! (a, b) {
   swap(a, b)
 }.
 
-Require Import bedrock2.WeakestPrecondition.
-Require Import bedrock2.Semantics bedrock2.FE310CSemantics.
+Require Import bedrock2.LeakageWeakestPrecondition.
+Require Import bedrock2.Semantics bedrock2.LeakageSemantics bedrock2.FE310CSemantics.
 Require Import coqutil.Map.Interface bedrock2.Map.Separation bedrock2.Map.SeparationLogic.
 
-Require bedrock2.WeakestPreconditionProperties.
+Require bedrock2.LeakageWeakestPreconditionProperties.
 From coqutil.Tactics Require Import Tactics letexists eabstract.
-Require Import bedrock2.ProgramLogic bedrock2.Scalars.
+Require Import bedrock2.LeakageProgramLogic bedrock2.Scalars.
 Require Import coqutil.Word.Interface.
 Require Import coqutil.Tactics.rdelta.
 
 Section WithParameters.
   Context {word: word.word 32} {mem: map.map word Byte.byte}.
   Context {word_ok: word.ok word} {mem_ok: map.ok mem}.
+  Context {pick_sp: PickSp}.
 
   Instance spec_of_swap : spec_of "swap" :=
-    fnspec! "swap" a_addr b_addr / a b R,
-    { requires t m := m =* scalar a_addr a * scalar b_addr b * R;
-      ensures T M :=  M =* scalar a_addr b * scalar b_addr a * R /\ T = t }.
+    fnspec! exists f, "swap" a_addr b_addr / a b R,
+    { requires k t m := m =* scalar a_addr a * scalar b_addr b * R;
+      ensures K T M :=  M =* scalar a_addr b * scalar b_addr a * R /\ T = t /\
+                          K = f a_addr b_addr ++ k }.
 
   Lemma swap_ok : program_logic_goal_for_function! swap.
-  Proof. repeat straightline; eauto. Qed.
+  Proof. repeat straightline. intuition eauto. align_trace. Qed.
 
   Instance spec_of_bad_swap : spec_of "bad_swap" :=
-    fnspec! "bad_swap" a_addr b_addr / a b R,
-    { requires t m := m =* scalar a_addr a * scalar b_addr b * R;
-      ensures T M :=  M =* scalar a_addr b * scalar b_addr a * R /\ T = t }.
+    fnspec! exists f, "bad_swap" a_addr b_addr / a b R,
+    { requires k t m := m =* scalar a_addr a * scalar b_addr b * R;
+      ensures K T M :=  M =* scalar a_addr b * scalar b_addr a * R /\ T = t /\
+                          K = f a_addr b_addr ++ k }.
   Lemma bad_swap_ok : program_logic_goal_for_function! bad_swap.
-  Proof. repeat straightline; eauto. Abort.
+  Proof. repeat straightline. intuition eauto; align_trace. Abort.
 
   Definition spec_of_swap_same : spec_of "swap" :=
     fnspec! "swap" a_addr b_addr / a R,
